theories/iris/examples/effects/coroutines_client.v
@@ -1,0 +1,449 @@
+
+From mathcomp Require Import ssreflect eqtype seq ssrbool.
+From iris.program_logic Require Import language.
+From iris.proofmode Require Import base tactics classes.
+From iris.base_logic Require Export gen_heap ghost_map proph_map.
+From iris.base_logic.lib Require Export fancy_updates.
+From iris.bi Require Export weakestpre.
+From iris.algebra Require Import auth excl.
+From Wasm Require Import type_checker_reflects_typing.
+From Wasm.iris.rules Require Export iris_rules iris_example_helper.
+From Wasm.iris.host Require Export iris_host.
+From Wasm.iris.examples.effects Require Import coroutines_module coroutines_implementation_code.
+
+
+Set Bullet Behavior "Strict Subproofs".
+Set Implicit Arguments.
+Unset Strict Implicit.
+Unset Printing Implicit Defensive.
+
+Section coroutines_client_functions.
+
+  Context `{!wasmG Σ, !hvisG Σ, !hmsG Σ, !hasG Σ}.
+  Context `{!inG Σ (one_shotR unitO)}.
+
+   Definition f1 :=
+     [ BI_const (xx 1);
+       BI_set_global 0;
+       BI_call 0;
+       BI_const (xx 1);
+       BI_set_global 1
+     ].
+
+   Definition f2 :=
+     [ BI_get_global 1;
+       BI_set_global 2;
+       BI_call 0;
+       BI_get_global 0;
+       BI_set_global 3
+     ].
+
+   Definition main :=
+     [ 
+       BI_ref_func 2;
+       BI_ref_func 3;
+       BI_call 1
+     ].
+
+
+   Definition wgpt a b :=
+     N.of_nat a ↦[wg] {| g_mut := MUT_mut ; g_val := xx b |}.
+   Definition wgpt_half a b :=
+     N.of_nat a ↦[wg]{ DfracOwn (1/2)%Qp } {| g_mut := MUT_mut ; g_val := xx b |}.
+   
+   Definition P1 addrx : iProp Σ :=
+     wgpt_half addrx 0.
+
+   Definition Q1 addrx : iProp Σ :=
+     wgpt_half addrx 1.
+
+   Definition P2 addra addrb : iProp Σ :=
+     ∃ a b, wgpt addra a ∗ wgpt addrb b. 
+
+   Definition Q2 addra addrb : iProp Σ :=
+     ∃ a b, wgpt addra a ∗ wgpt addrb b ∗ ⌜ a = 1 -> b = 1 ⌝ .
+
+   Definition I addrx addry : iProp Σ :=
+     (wgpt_half addrx 0 ∗ wgpt addry 0) ∨
+       (wgpt_half addrx 1 ∗ wgpt addry 0) ∨
+       (wgpt_half addrx 1 ∗ wgpt addry 1).
+
+   Definition spec_f1 f Ψ addr_f1 cl_f1 addrx addry addr_yield cl_yield: iProp Σ :=
+     □ (N.of_nat addr_f1 ↦[wf] cl_f1 -∗
+        N.of_nat addr_yield ↦[wf] cl_yield -∗
+         P1 addrx -∗
+         I addrx addry -∗
+              EWP [AI_invoke addr_f1] UNDER f <| Ψ |> {{ v; f' ,
+                  ⌜ v = immV [] ⌝ ∗
+                  ⌜ f' = f ⌝ ∗
+                  N.of_nat addr_f1 ↦[wf] cl_f1 ∗
+                  N.of_nat addr_yield ↦[wf] cl_yield ∗
+                  Q1 addrx ∗
+                  I addrx addry
+       }})%I.
+   
+   Definition spec_f2 f Ψ addr_f2 cl_f2 addrx addry addra addrb addr_yield cl_yield: iProp Σ :=
+     □ (N.of_nat addr_f2 ↦[wf] cl_f2 -∗
+          N.of_nat addr_yield ↦[wf] cl_yield -∗
+          P2 addra addrb -∗
+          I addrx addry -∗
+             EWP [AI_invoke addr_f2] UNDER f <| Ψ |> {{ v; f' ,
+                ⌜ v = immV [] ⌝ ∗
+                ⌜ f' = f ⌝ ∗
+                N.of_nat addr_f2 ↦[wf] cl_f2 ∗
+                N.of_nat addr_yield ↦[wf] cl_yield ∗
+                Q2 addra addrb ∗
+                I addrx addry }})%I.
+
+   Definition spec_main f Ψ addr_main cl_main addrx addry addra addrb addr_yield cl_yield addr_par cl_par addr_f1 cl_f1 addr_f2 cl_f2: iProp Σ :=
+     □ (N.of_nat addr_main ↦[wf] cl_main -∗
+             N.of_nat addr_f1 ↦[wf] cl_f1 -∗
+             N.of_nat addr_f2 ↦[wf] cl_f2 -∗
+             N.of_nat addr_yield ↦[wf] cl_yield -∗
+             N.of_nat addr_par ↦[wf] cl_par -∗
+             (∃ x y a b, wgpt addrx x ∗ wgpt addry y ∗ wgpt addra a ∗ wgpt addrb b) -∗
+                EWP [AI_invoke addr_main] UNDER f <| Ψ |> {{ v; f' ,
+                     ⌜ v = immV [] ⌝ ∗
+                     ⌜ f' = f ⌝ ∗
+                     N.of_nat addr_main ↦[wf] cl_main ∗
+                     N.of_nat addr_f1 ↦[wf] cl_f1 ∗
+                     N.of_nat addr_f2 ↦[wf] cl_f2 ∗
+                     N.of_nat addr_yield ↦[wf] cl_yield ∗
+                     N.of_nat addr_par ↦[wf] cl_par ∗
+                     Q2 addra addrb }})%I.
+
+
+  Definition client_inst addr_yield addr_par addr_f1 addr_f2 addr_main addrx addry addra addrb :=
+    {| inst_types := [ emptyt; par_type ];
+      inst_funcs := [ addr_yield; addr_par; addr_f1; addr_f2; addr_main ] ;
+      inst_tab := [];
+      inst_memory := [];
+      inst_globs := [addrx; addry; addra; addrb];
+      inst_tags := [] |}.
+   
+   Lemma spec_f1_proof f Ψ addr_f1 cl_f1 addrx addry addr_yield cl_yield addr_par addr_f2 addr_main addra addrb :
+     cl_f1 = FC_func_native (client_inst addr_yield addr_par addr_f1 addr_f2 addr_main addrx addry addra addrb) emptyt [] f1 ->
+     yield_spec addr_yield cl_yield Ψ (I addrx addry)
+       ⊢ spec_f1 f Ψ addr_f1 cl_f1 addrx addry addr_yield cl_yield.
+   Proof.
+     iIntros (->) "#Hyield !> Hwf1 Hwfyield HP1 HI".
+     rewrite - (app_nil_l [AI_invoke addr_f1]).
+     iApply (ewp_invoke_native with "Hwf1").
+     done. done. done.
+     iIntros "!> Hwf1".
+     iApply ewp_frame_bind.
+     done. done.
+     iSplitR; last first.
+     iSplitR "Hwf1".
+     rewrite -(app_nil_l [AI_basic _]).
+     iApply ewp_block.
+     done. done. done. done.
+     iApply (ewp_label_bind with "[-]").
+     2:{ iPureIntro.
+         instantiate (5 := []).
+         rewrite /lfilled /lfill /= app_nil_r //. }
+     rewrite separate2.
+     iApply ewp_seq.
+     done.
+     iSplitR; last first.
+     iAssert (wgpt addrx 0 ∗ wgpt addry 0)%I with "[HI HP1]" as "[Hx Hy]".
+     { iDestruct "HI" as "[[Hx Hy] | [[Hx Hy] | [Hx Hy]]]".
+       iFrame.
+       all: iDestruct (pointsto_agree with "Hx HP1") as "%Habs" => //. } 
+     iSplitL "Hx".
+     iApply (ewp_set_global with "[] Hx").
+     done.
+     auto_instantiate.
+     2: by iIntros (?) "[[% _] _]".
+     iIntros (??) "[[-> ->] Hx]".
+     iSimpl.
+     rewrite (separate1 (AI_basic _)).
+     iApply ewp_seq.
+     done.
+     iSplitR; last first.
+     simpl.
+     iDestruct "Hx" as "[Hx1 Hx2]".
+     iSplitR "Hx2".
+     iApply ewp_call.
+     done.
+     iApply ("Hyield" with "[Hx1 Hy] Hwfyield").
+     simpl.
+     iRight. iLeft. iFrame.
+     iIntros (??) "(-> & -> & HI & Hwfyield)".
+     iSimpl.
+     iAssert (wgpt addrx 1 ∗ ∃ i, wgpt addry i)%I with "[HI Hx2]" as "(Hx & %i & Hy)".
+
+     { iDestruct "HI" as "[[Hx Hy] | [[Hx Hy] | [Hx Hy]]]".
+       iDestruct (pointsto_agree with "Hx Hx2") as %Habs => //.
+       all: iFrame. }
+     iApply (ewp_wand with "[Hy]").
+     iApply (ewp_set_global with "[] Hy").
+     done.
+     auto_instantiate.
+     2: by iIntros (?) "[% _]".
+     iIntros (??) "[[-> ->] Hy]".
+     simpl.
+     iIntros (LI HLI).
+     move/lfilledP in HLI; inversion HLI; subst.
+     inversion H8; subst.
+     iSimpl.
+     iApply ewp_label_value.
+     done.
+     instantiate (1 := λ v f,  (⌜ v = immV _ ⌝ ∗ ⌜ f = Build_frame _ _ ⌝ ∗ _)%I).
+     iSplitR; first done.
+     iSplitR; first done.
+     iCombine "Hwfyield Hx Hy" as "H".
+     iExact "H".
+     iIntros (??) "(-> & -> & Hwfyield & Hx & Hy)".
+     iApply ewp_frame_value.
+     done. done.
+     iSplit; first done.
+     iSplit; first done.
+     iFrame.
+     iDestruct "Hx" as "[Hx1 Hx2]".
+     iFrame.
+     iRight. iRight.
+     iFrame.
+     iIntros (?) "[% _]" => //.
+   Qed. 
+     
+   Lemma spec_f2_proof f Ψ addr_f2 cl_f2 addrx addry addr_yield cl_yield addr_par addr_f1 addr_main addra addrb :
+     cl_f2 = FC_func_native (client_inst addr_yield addr_par addr_f1 addr_f2 addr_main addrx addry addra addrb) emptyt [] f2 ->
+     yield_spec addr_yield cl_yield Ψ (I addrx addry)
+       ⊢ spec_f2 f Ψ addr_f2 cl_f2 addrx addry addra addrb addr_yield cl_yield.
+   Proof.
+     iIntros (->) "#Hyield !> Hwf2 Hwfyield HP2 HI".
+     iDestruct "HP2" as (a b) "[Ha Hb]".
+     iDestruct "HI" as "[[Hx Hy] | [[Hx Hy] | [Hx Hy]]]".
+     - (* Case 1 *) 
+       rewrite - (app_nil_l [AI_invoke addr_f2]).
+       iApply (ewp_invoke_native with "Hwf2").
+       done. done. done.
+       iIntros "!> Hwf2".
+       iApply ewp_frame_bind.
+       done. done.
+       iSplitR; last first.
+       iSplitR "Hwf2".
+       rewrite -(app_nil_l [AI_basic _]).
+       iApply ewp_block.
+       done. done. done. done.
+       iApply (ewp_label_bind with "[-]").
+       2:{ iPureIntro.
+           instantiate (5 := []).
+           rewrite /lfilled /lfill /= app_nil_r //. }
+       rewrite (separate1 (AI_basic _)).
+       iApply ewp_seq.
+       done.
+       iSplitR; last first.
+       iSplitL "Hy".
+       iApply (ewp_get_global with "[] Hy").
+       done. done.
+       iSimpl.
+       auto_instantiate.
+       2: by iIntros (?) "[[% _] _]".
+       iIntros (??) "[[->->] Hy]".
+       iSimpl.
+       rewrite separate2.
+       iApply ewp_seq.
+       done.
+       iSplitR; last first.
+       iSplitL "Ha".
+       iApply (ewp_set_global with "[] Ha").
+       done.
+       auto_instantiate.
+       2: by iIntros (?) "[[% _] _]".
+       iIntros (??) "[[-> ->] Ha]".
+       iSimpl.
+       rewrite (separate1 (AI_basic _)).
+       iApply ewp_seq.
+       done.
+       iAssert (I addrx addry)%I with "[Hx Hy]" as "HI".
+       by iLeft; iFrame.
+       iSplitR; last first.
+       iSplitL "HI Hwfyield".
+       iApply ewp_call.
+       done.
+       iApply ("Hyield" with "HI Hwfyield").
+       2: by iIntros (?) "[% _]".
+       iIntros (??) "(-> & -> & HI & Hwfyield)".
+       iDestruct "HI" as "[[Hx Hy] | [[ Hx Hy ] | [Hx Hy]]]".
+
+       iSimpl.
+        rewrite (separate1 (AI_basic _)).
+        iApply ewp_seq.
+        try done.
+        iSplitR; last first.
+        try iSplitL "Hx".
+        try iApply (ewp_get_global with "[] Hx").
+        try done.
+        try by auto_instantiate.
+        try by iIntros (?) "[[% _] _]".
+        iIntros (??) "[[-> ->] Hx]".
+        iSimpl.
+        iApply (ewp_wand with "[Hb]").
+        try iApply (ewp_set_global with "[] Hb").
+        try done.
+        try auto_instantiate.
+        iIntros (??) "[[-> ->] Hb]".
+        iIntros (LI HLI).
+        move/lfilledP in HLI; inversion HLI; subst.
+        inversion H8; subst.
+        iApply ewp_label_value.
+        try done.
+       instantiate (1 := λ v f, (⌜ v = immV _ ⌝ ∗ ⌜ f = Build_frame _ _ ⌝ ∗ _ ∗ (_ ∨ _ ∨ _ ∨ _ ∨ _ ∨ _ ∨ _ ∨ _ ∨ _))%I).
+        iSplit; first done.
+        iSplit; first done.
+        iSplitL "Hwfyield"; first iExact "Hwfyield".
+        iCombine "Ha Hb Hx Hy" as "H".
+       iLeft; iExact "H".
+        iRight.
+       iLeft; iExact "H".
+        iRight.
+       iLeft; iExact "H".
+        iRight.
+       iLeft; iExact "H".
+        iRight.
+       iLeft; iExact "H".
+        iRight.
+       iLeft; iExact "H".
+        iRight.
+       iLeft; iExact "H".
+        iRight.
+       iLeft; iExact "H".
+       iRight.
+       iExact "H".
+     }
+     2: by iIntros (?) "[% _]".
+     iIntros (??) "(-> & -> & Hwfyield & H)".
+     iApply ewp_frame_value.
+     done. done.
+     iSplit; first done.
+     iSplit; first done.
+     iFrame.
+     iDestruct "H" as "[ (Ha & Hb & Hx & Hy) | [ (Ha & Hb & Hx & Hy) | [ (Ha & Hb & Hx & Hy) | [ (Ha & Hb & Hx & Hy) | [ (Ha & Hb & Hx & Hy) | [ (Ha & Hb & Hx & Hy) | [ (Ha & Hb & Hx & Hy) | [ (Ha & Hb & Hx & Hy) | (Ha & Hb & Hx & Hy) ]]]]]]]]".
+     all: iFrame.
+     all: iSplit; first try done.
+       
+       
+
+     
+
+
+End coroutines_client_functions.
+
+Section coroutines_client_module.
+
+  Context `{!wasmG Σ, !hvisG Σ, !hmsG Σ, !hasG Σ}.
+
+  Definition client_module :=
+    {|
+      mod_types := [ emptyt; par_type ];
+      mod_funcs :=
+      [ {|
+          modfunc_type := Mk_typeidx 0 ;
+          modfunc_locals := [] ;
+          modfunc_body := f1
+        |};
+        {|
+          modfunc_type := Mk_typeidx 0 ;
+          modfunc_locals := [] ;
+          modfunc_body := f2
+        |};
+        {|
+          modfunc_type := Mk_typeidx 0;
+          modfunc_locals := [];
+          modfunc_body := main
+        |} 
+      ] ;
+      mod_tables := [];
+      mod_mems := [] ;
+      mod_globals := [
+        {| modglob_type := {| tg_mut := MUT_mut ; tg_t := T_i32 |} ;
+          modglob_init := [BI_const (xx 0)] |};
+        {| modglob_type := {| tg_mut := MUT_mut ; tg_t := T_i32 |} ;
+          modglob_init := [BI_const (xx 0)] |};
+        {| modglob_type := {| tg_mut := MUT_mut ; tg_t := T_i32 |} ;
+          modglob_init := [BI_const (xx 0)] |};
+        {| modglob_type := {| tg_mut := MUT_mut ; tg_t := T_i32 |} ;
+          modglob_init := [BI_const (xx 0)] |}
+      ];
+      mod_elem := [] ;
+      mod_data := [] ;
+      mod_start := Some {| modstart_func := Mk_funcidx 4 |} ; 
+      mod_imports := [
+        {| imp_module := String.list_byte_of_string "coroutines module";
+          imp_name := String.list_byte_of_string "yield function";
+          imp_desc := ID_func 0
+        |};
+        {| imp_module := String.list_byte_of_string "coroutines module";
+          imp_name := String.list_byte_of_string "par function";
+          imp_desc := ID_func 1
+        |}
+      ];
+      mod_exports := [];
+      mod_tags := []
+    |}.
+
+  Definition impts := [ET_func emptyt ; ET_func par_type].
+
+  Lemma client_module_typing :
+    module_typing client_module impts [].
+  Proof.
+    unfold module_typing.
+    exists [emptyt; emptyt; emptyt], (repeat {| tg_mut := MUT_mut ; tg_t := T_i32 |} 4).
+    simpl.
+    repeat split; eauto.
+    - constructor; last constructor; last constructor; last constructor.
+      all: cbn; repeat split => //.
+      + apply/b_e_type_checker_reflects_typing.
+        simpl. done.
+      + apply/b_e_type_checker_reflects_typing.
+        simpl. done.
+      + apply/b_e_type_checker_reflects_typing.
+        simpl. done.
+    - constructor; last constructor; last constructor; last constructor; last constructor.
+      all: cbn; repeat split => //.
+      all: constructor.
+    - constructor; last constructor; last constructor.
+      all: cbn; apply/andP; split => //.
+  Qed.
+
+
+  Definition client_module_instantiate yield_exp_addr par_exp_addr mod_addr mod_addr' :=
+    [ ID_instantiate [ yield_exp_addr ; par_exp_addr ] mod_addr [] ;
+      ID_instantiate [] mod_addr' [ yield_exp_addr ; par_exp_addr ]
+    ].
+
+  Notation "{{{{ P }}}} es {{{{ v , Q }}}}" :=
+    (□ ∀ Φ, P -∗ (∀ v, Q -∗ Φ v) -∗ WP (es : host_expr) @ NotStuck ; ⊤ {{ v, Φ v }})%I (at level 50).
+
+  Lemma instantiate_client yield_exp_addr par_exp_addr mod_addr mod_addr' : 
+    
+    ⊢ {{{{ 
+              mod_addr ↪[mods] coroutines_module ∗
+                mod_addr' ↪[mods] client_module ∗
+                (∃ exp1, yield_exp_addr ↪[vis] exp1) ∗
+                (∃ exp2, par_exp_addr ↪[vis] exp2)
+      }}}}
+      ((client_module_instantiate yield_exp_addr par_exp_addr mod_addr mod_addr',
+         [], empty_frame) : host_expr) 
+        {{{{  x,  ⌜x = (immHV [], empty_frame)⌝ ∗
+                         mod_addr ↪[mods] coroutines_module ∗
+                         mod_addr' ↪[mods] client_module ∗
+                         ∃ inst addra addrb addrx addry vala valb valx valy addr_f1 cl_f1 addr_f2 cl_f2 addr_main cl_main,
+                           wgpt addra valb ∗
+                             wgpt addrb valb ∗
+                             wgpt addrx valx ∗
+                             wgpt addry valy ∗
+                             ⌜ vala = 1 -> valb = 1 ⌝ ∗
+                            N.of_nat addr_f1 ↦[wf] cl_f1 ∗
+                            N.of_nat addr_f2 ↦[wf] cl_f2 ∗
+                            N.of_nat addr_main ↦[wf] cl_main ∗
+                            
+                         
+        }}}} .
+  Proof.
+      
+
+   
+     
